src/syncablep.lean
@@ -1,0 +1,27 @@
+import parlang
+
+open parlang
+
+section
+
+variables {n : ℕ} {σ : Type} {ι : Type} {τ : ι → Type} [decidable_eq ι]
+
+/-- syncable with the exception that no threads is allowed to store 
+or load in stores and loads respectively -/
+def syncable' (stores : list ι) (loads : list ι) (s : state n σ τ) (m : memory τ) : Prop :=
+(∀i:ι,
+    (∀ tid, i ∉ (s.threads.nth tid).stores ∧ m i = (s.threads.nth tid).global i) ∨
+    (∃ tid, i ∈ (s.threads.nth tid).stores ∧ m i = (s.threads.nth tid).global i ∧
+        (∀ tid', tid ≠ tid' → i ∉ (s.threads.nth tid').accesses))) ∧
+(∀ i tid, i ∈ stores → i ∉ (s.threads.nth tid).stores) ∧
+(∀ i tid, i ∈ loads → i ∉ (s.threads.nth tid).loads)
+
+example (s : state n σ τ) (m : memory τ) : syncable' [] [] s m ↔ state.syncable s m := begin
+    unfold syncable',
+    simp,
+    refl,
+end
+
+
+
+end
